Parameterize over dereference_scalar in more places
This will allow us to reuse the same code to load inputs and outputs,
when we want to enforce the spec of reading back and removing all of the
values and then saying that the resulting symbolic memory state is
empty.

Some of the proofs are not quite as complete as they were before, but I
hope to replace them soon with a more principled approach.

src/Assembly/Equivalence.v
@@ -122,7 +122,7 @@ printing functions on command-lines options indicating how verbose to
 be in printing the error message. *)
 Inductive EquivalenceCheckingError :=
 | Symbolic_execution_failed (_ : Symbolic.error) (_ : symbolic_state)
-| Internal_error_output_load_failed (_ : list (option idx)) (_ : symbolic_state)
+| Internal_error_output_load_failed (_ : list ((REG + idx) + idx)) (_ : symbolic_state)
 | Internal_error_extra_input_arguments (t : API.type) (unused_arguments : list (idx + list idx))
 | Not_enough_registers (num_given num_extra_needed : nat)
 | Registers_too_narrow (bad_reg : list REG)
@@ -628,18 +628,24 @@ Definition build_merge_array_addresses (base : idx) (items : list idx) : M (list
               (fun s => Success (addr, update_mem_with s (cons (addr,idx)))))
           )%x86symex (List.enumerate items).
 
-Fixpoint build_merge_base_addresses (items : list (idx + list idx)) (reg_available : list REG) : M (list (option idx))
+Fixpoint build_merge_base_addresses {dereference_scalar:bool} (items : list (idx + list idx)) (reg_available : list REG) : M (list ((REG + idx) + idx))
   := match items, reg_available with
      | [], _ | _, [] => Symbolic.ret []
      | inr idxs :: xs, r :: reg_available
        => (base <- SetRegFresh r; (* note: overwrites initial value *)
            addrs <- build_merge_array_addresses base idxs; (* note: overwrites initial value *)
-           rest <- build_merge_base_addresses xs reg_available;
-           Symbolic.ret (Some base :: rest))
+           rest <- build_merge_base_addresses (dereference_scalar:=dereference_scalar) xs reg_available;
+           Symbolic.ret (inr base :: rest))
      | inl idx :: xs, r :: reg_available =>
-          (_ <- SetReg r idx; (* note: overwrites initial value *)
-           rest <- build_merge_base_addresses xs reg_available;
-           Symbolic.ret (None :: rest))
+          (addr <- (if dereference_scalar
+                    then
+                      (addr <- SetRegFresh r;
+                       fun s => Success (inr addr, update_mem_with s (cons (addr, idx))))
+                    else
+                      (_ <- SetReg r idx; (* note: overwrites initial value *)
+                       ret (inl r)));
+           rest <- build_merge_base_addresses (dereference_scalar:=dereference_scalar) xs reg_available;
+           Symbolic.ret (inl addr :: rest))
      end%N%x86symex.
 
 Fixpoint dag_gensym_n (n : nat) : dag.M (list symbol) :=
@@ -1057,12 +1063,15 @@ Definition init_symbolic_state (d : dag) : symbolic_state
        symbolic_flag_state := Tuple.repeat None 6;
      |}.
 
+Definition compute_stack_base (stack_size : nat) : M idx
+  := (rsp_val <- SetRegFresh rsp;
+      stack_size <- Symbolic.App (zconst 64 (-8 * Z.of_nat stack_size), []);
+      Symbolic.App (add 64%N, [rsp_val; stack_size]))%x86symex.
+
 Definition build_merge_stack_placeholders (stack_size : nat)
   : M unit
   := (stack_placeholders <- lift_dag (build_inputarray stack_size);
-      rsp_val <- SetRegFresh rsp;
-      stack_size <- Symbolic.App (zconst 64 (-8 * Z.of_nat stack_size), []);
-      stack_base <- Symbolic.App (add 64%N, [rsp_val; stack_size]);
+      stack_base <- compute_stack_base stack_size;
       _ <- build_merge_array_addresses stack_base stack_placeholders;
       ret tt)%x86symex.
 
@@ -1072,15 +1081,24 @@ Definition LoadArray (base : idx) (len : nat) : M (list idx)
               Load64 addr)%x86symex)
           (seq 0 len).
 
-Definition LoadOutputs (outputaddrs : list (option idx)) (output_types : type_spec)
+Definition LoadOutputs {dereference_scalar:bool} (outputaddrs : list ((REG + idx) + idx)) (output_types : type_spec)
   : M (list (idx + list idx))
-  := (asm_output <- mapM (fun '(ocells, spec) =>
+  := (mapM (fun '(ocells, spec) =>
             match ocells, spec with
-            | None, None | None, Some _ | Some _, None => err (error.load 0)
-            | Some base, Some len
-              => LoadArray base len
-            end) (List.combine outputaddrs output_types);
-      Symbolic.ret (List.map inr asm_output))%N%x86symex.
+            | inl _, Some _ | inr _, None => err (error.load 0)
+            | inl addr, None
+              => (v <- match addr, dereference_scalar with
+                       | inl r, false
+                         => GetReg r
+                       | inr addr, true
+                         => Load64 addr
+                       | inl _, true | inr _, false => err (error.load 0)
+                       end;
+                  ret (inl v))
+            | inr base, Some len
+              => (v <- LoadArray base len;
+                  ret (inr v))
+            end) (List.combine outputaddrs output_types))%N%x86symex.
 
 Definition symex_asm_func_M
            (callee_saved_registers : list REG)
@@ -1088,15 +1106,15 @@ Definition symex_asm_func_M
            (inputs : list (idx + list idx)) (reg_available : list REG) (asm : Lines)
   : M (ErrorT EquivalenceCheckingError (list (idx + list idx)))
   := (output_placeholders <- lift_dag (build_inputs output_types);
-      argptrs <- build_merge_base_addresses (output_placeholders ++ inputs) reg_available;
+      argptrs <- build_merge_base_addresses (dereference_scalar:=false) (output_placeholders ++ inputs) reg_available;
       _ <- build_merge_stack_placeholders stack_size;
       initial_register_values <- mapM GetReg callee_saved_registers;
       _ <- SymexLines asm;
       final_register_values <- mapM GetReg callee_saved_registers;
       let unsaved_registers : list (REG * (idx * idx)) := List.filter (fun '(r, (init, final)) => negb (init =? final)%N) (List.combine callee_saved_registers (List.combine initial_register_values final_register_values)) in
-      let outputaddrs : list (option idx) := firstn (length argptrs - length inputs) argptrs in
+      let outputaddrs : list (_ + idx) := firstn (length argptrs - length inputs) argptrs in
       (* In the following line, we match on the result so we can emit Internal_error_output_load_failed in the calling function, rather than passing through the placeholder error from LoadOutputs *)
-      (fun s => match LoadOutputs outputaddrs output_types s, unsaved_registers with
+      (fun s => match LoadOutputs (dereference_scalar:=false) outputaddrs output_types s, unsaved_registers with
                 | Success (asm_output, s), []
                   => Success (Success asm_output, s)
                 | Error (_, s), _
